feat: intrinsically typed variables

EffectSSA/Syntax/Typed/Basic.lean
@@ -1,4 +1,5 @@
 import EffectSSA.Syntax.Untyped
+import EffectSSA.Syntax.Typed.TVar
 import EffectSSA.Types
 
 /-!
@@ -7,25 +8,59 @@ We define typed variants of syntax datastructure, which bundle an untyped
 datastructer with a proof of well-typedness
 -/
 namespace EffectSSA
-variable {τ} [MemorySignature τ]
+variable {τ}
 
 structure TInstruction (Γ : Context τ) (Δ : Context τ) where
   instruction : Instruction τ
-  wt : instruction.WellTyped Γ Δ
+  wt : instruction.WellTyped Γ Δ := by grind
 
 structure TInstructionSeq (Γ : Context τ) (Δ : Context τ) where
   seq : InstructionSeq τ
-  wt : seq.WellTypedWith Γ Δ
+  wt : seq.WellTypedWith Γ Δ := by grind
 
 structure TProgram (Γ : Context τ) (ts : List τ.Typ) where
   program : Program τ
-  wt : program.WellTyped Γ ts
+  wt : program.WellTyped Γ ts := by grind
+
+/-!
+## Coercions
+--------------------------------------------------------------------------------
+The typed structures can be implicitly coerced into the underlying
+untyped variants
+-/
+variable {Γ : Context τ}
+
+instance : CoeOut (TInstruction Γ Δ) (Instruction τ) where coe := TInstruction.instruction
+instance : CoeOut (TInstructionSeq Γ Δ) (InstructionSeq τ) where coe := TInstructionSeq.seq
+instance : CoeOut (TProgram Γ ts) (Program τ) where coe := TProgram.program
+
+/-!
+## Grind Attributes
+--------------------------------------------------------------------------------
+-/
+
+attribute [grind! .] TInstruction.wt
+attribute [grind! .] TInstructionSeq.wt
+attribute [grind! .] TProgram.wt
 
 /-!
 ## Definitions
 --------------------------------------------------------------------------------
 -/
 variable {Γ : Context τ} {ts : List τ.Typ}
+
+/-!
+### Constructors
+-/
+
+def TInstructionSeq.nil (Γ : Context τ) : TInstructionSeq Γ Γ where seq := .nil
+def TInstructionSeq.cons (i : TInstruction Γ Δ) (is : TInstructionSeq Δ Ξ) :
+    TInstructionSeq Γ Ξ where
+  seq := i ;> is
+
+/-!
+### Projections
+-/
 
 /-- The (internal) context after executing the instruction sequence of `p`. -/
 @[grind =]
@@ -36,3 +71,48 @@ noncomputable def TProgram.returnContext (p : TProgram Γ ts) : Context τ :=
 def TProgram.instructions (p : TProgram Γ ts) : TInstructionSeq Γ p.returnContext where
   seq := p.program.instructions
   wt := by grind
+
+def TProgram.returnVars (p : TProgram Γ ts) : TVarList Γ ts where
+  vs := ⟨p.program.returnVars, by grind⟩
+  wt := by
+    intro i;
+    have ⟨_, _, _, len_eq, wt⟩ := p.wt
+    specialize wt i.val (by grind)
+    /-
+    FIXME: proving this will likely be nicer with some theory around context
+    "extensions". I.e., we likely want some API which allows us to conclude
+    that context `Δ` "extends" `Γ` from `Γ ⊢ ... :: Δ`, which in turn will
+    let us know that `Δ[v]? = some t` implies `Γ[v]? = some t`.
+    If we had such API, the following sorry ought to be provable by grind.
+    -/
+    sorry
+
+/-!
+## Lemmas
+--------------------------------------------------------------------------------
+-/
+
+@[simp, grind =] theorem TInstructionSeq.seq_nil : (nil Γ).seq = .nil := by rfl
+@[simp, grind =] theorem TInstructionSeq.seq_cons :
+  (cons i is).seq = i.instruction ;> is.seq := by rfl
+
+
+/-!
+## Induction Principles
+--------------------------------------------------------------------------------
+FIXME: For now, let's just do induction, no data-producing recursion yet!
+-/
+
+@[elab_as_elim, induction_eliminator]
+def TInstructionSeq.indOn {motive : ∀ {Γ Δ : Context τ}, TInstructionSeq Γ Δ → Prop}
+    {Γ Δ} (is : TInstructionSeq Γ Δ)
+    (nil : ∀ Γ, motive (.nil Γ))
+    (cons : ∀ {Γ Δ Ξ} (i : TInstruction Γ Δ) (is : TInstructionSeq Δ Ξ),
+      motive is → motive (.cons i is)) :
+    motive is :=
+  match is with
+  | ⟨.nil, .nil h_eq⟩ => h_eq ▸ (nil _)
+  | ⟨i ;> is, .cons wt_i wt_is⟩ =>
+      let i : TInstruction Γ _ := ⟨i, wt_i⟩
+      let is : TInstructionSeq _ Δ := ⟨is, wt_is⟩
+      cons i is (indOn is nil cons)
