EffectSSA/Syntax/Typed/TVar.lean
@@ -1,0 +1,51 @@
+import EffectSSA.Syntax.Untyped
+import EffectSSA.Types
+
+/-!
+# Intrinsically Well-typed Variables
+-/
+namespace EffectSSA
+variable {τ}
+
+/--
+`TVar Γ t` is a variable which is guaranteed to be assigned
+type `t` in context `Γ`.
+-/
+structure TVar (Γ : Context τ) (t : τ.Typ) where
+  ofVar ::
+    toVar : Var
+    wt : Γ[toVar]? = some t := by grind
+
+/--
+`vs : TVarList Γ ts` is a list of variables, such that `vs[i]`
+is assinged the respective type `ts[i]` in `Γ`.
+-/
+structure TVarList (Γ : Context τ) (ts : List τ.Typ) where
+  vs : List.Vector Var ts.length
+  wt : ∀ (i : Fin ts.length), Γ[vs[i]]? = some ts[i] := by grind
+
+/-!
+## Coercions
+--------------------------------------------------------------------------------
+The typed structures can be implicitly coerced into the underlying
+untyped variants
+-/
+variable {Γ : Context τ}
+
+instance : CoeOut (TVar Γ t) Var where coe := TVar.toVar
+
+/-!
+## Grind Attributes
+--------------------------------------------------------------------------------
+-/
+
+grind_pattern TVar.wt => TVar.toVar self
+attribute [grind =] TVarList.wt
+
+/-!
+## TVarList Accessor
+--------------------------------------------------------------------------------
+-/
+
+def TVarList.get (vs : TVarList Γ ts) (i : Fin ts.length) : TVar Γ ts[i] :=
+  .ofVar vs.vs[i]
